lakefile.lean
@@ -18,9 +18,9 @@ lean_lib E3 {
 
 }
 
-require mathlib from git "https://github.com/leanprover-community/mathlib4.git" @ "9837ca9d65d9de6fad1ef4381750ca688774e608"
+require mathlib from git "https://github.com/leanprover-community/mathlib4.git" @ "v4.19.0"
 
-require smt from git "https://github.com/ufmg-smite/lean-smt.git" @ "9b81e91cc9ea3833203317a7f425267112083672"
+require smt from git "https://github.com/vasnesterov/lean-smt" @ "main"
 
 def tmpFileDir := "tmp"
 
@@ -66,4 +66,4 @@ require checkdecls from git "https://github.com/PatrickMassot/checkdecls.git"
 
 meta if get_config? env = some "dev" then
 require «doc-gen4» from git
-  "https://github.com/leanprover/doc-gen4.git" @ "v4.15.0"
+  "https://github.com/leanprover/doc-gen4.git" @ "v4.19.0"
